generalizing monotonic seq with an seq refinement (not pushed yet in fstar)

src/tls/Concrete.fst
@@ -4,3 +4,4 @@ let ideal_Nonce = false
 let ideal_Sig = false 
 let ideal_PMS = false 
 let ideal_PRF = false 
+let ideal_AEAD = false
