src/tls/Ideal.fst
@@ -4,3 +4,4 @@ assume val ideal_Nonce : bool
 assume val ideal_Sig : bool 
 assume val ideal_PMS : bool 
 assume val ideal_PRF : bool 
+assume val ideal_AEAD: bool
