src/tls/StreamAE.fst
@@ -4,6 +4,9 @@ module StreamAE
 // plaintexts; concretely, we use AES_GCM but any other AEAD algorithm
 // would do.
 
+// This implementations *assumes* "Stateful AE" security, then calls CoreCrypto
+// Alternatively, we should go down to AEAD with noAD. 
+
 open FStar.Heap
 open FStar.HyperHeap
 open FStar.Seq
@@ -26,7 +29,10 @@ let gen parent i =
   let writer_r = new_region parent in
   if authId i then 
     let log : ideal_log writer_r i = alloc_mref_seq writer_r Seq.createEmpty in
-    let ectr: ideal_ctr writer_r i log = new_counter writer_r 0 log in
+    let h = ST.get() in
+    assert(0 <= max_ctr); 
+    assert(0 <= Seq.length (m_sel #writer_r #(s:seq (entry i){True}) h log));
+    let ectr: ideal_ctr writer_r i log = new_seqn writer_r 0 max_ctr log in
     State #i #Writer #writer_r #writer_r kv iv log ectr
   else 
     let ectr: concrete_ctr writer_r i = m_alloc writer_r 0 in
@@ -38,7 +44,7 @@ let genReader parent #i w =
   if authId i
   then
     let log : ideal_log w.region i = w.log in
-    let dctr: ideal_ctr reader_r i log = new_counter reader_r 0 log in
+    let dctr: ideal_ctr reader_r i log = new_seqn reader_r 0 max_ctr log in
     State #i #Reader #reader_r #(w.region) w.key w.iv w.log dctr
   else let dctr : concrete_ctr reader_r i = m_alloc reader_r 0 in
     State #i #Reader #reader_r #(w.region) w.key w.iv () dctr
@@ -60,7 +66,7 @@ let leak #i #role s = State.key s, State.iv s
 //
 // The XORing is a fixed, ad hoc, random permutation; not sure what is gained;
 // we can reason about sequence-number collisions before applying it.
-let aeIV i (seqn:counter) (staticIV:iv i) : lbytes (iv_length i) =
+let aeIV i (seqn:seqnum) (staticIV:iv i) : lbytes (iv_length i) =
   lemma_repr_bytes_values seqn;
   max_ctr_value ();
   let extended = bytes_of_int (iv_length i) seqn in
@@ -74,7 +80,7 @@ let noAD = empty_bytes
    safeId i is fixed to false and after removal of the cryptographic ghost log,
    i.e. all idealization is turned off *)
 let encrypt #i e l p =
-  let ctr = ctr e.counter in 
+  let ctr = ctr e.seqn in 
   m_recall ctr;
   let text = if safeId i then createBytes l 0z else repr i l p in
   let n = m_read ctr in
@@ -84,32 +90,31 @@ let encrypt #i e l p =
     begin
     let ilog = ilog e.log in
     m_recall ilog;
-    let ictr: ideal_ctr e.region i ilog = e.counter in
-    testify_counter ictr;
-    write_at_end ilog (Entry l c p); //need to extend the log first, before incrementing the counter for monotonicity; do this only if ideal
+    let ictr: ideal_ctr e.region i ilog = e.seqn in
+    testify_seqn ictr;
+    write_at_end ilog (Entry l c p); //need to extend the log first, before incrementing the seqn for monotonicity; do this only if ideal
     m_recall ictr;
-    increment_counter ictr;
+    increment_seqn (fun _ -> True) ictr;
     m_recall ictr
     end
   else
     m_write ctr (n + 1);
   c
 
-
-// decryption, idealized as a lookup of (c,ad) in the log for safe instances
+// decryption, idealized as a lookup at index d.seq# in the log for safe instances
 let decrypt #i d l c =
-  let ctr = ctr d.counter in 
+  let ctr = ctr d.seqn in 
   m_recall ctr;
   let j = m_read ctr in
   if authId i 
   then 
     let ilog = ilog d.log in
     let log  = m_read ilog in
-    let ictr: ideal_ctr d.region i ilog = d.counter in
-    let _ = testify_counter ictr in //now we know that j <= Seq.length log
+    let ictr: ideal_ctr d.region i ilog = d.seqn in
+    let _ = testify_seqn ictr in //now we know that j <= Seq.length log
     if j < Seq.length log && matches l c (Seq.index log j) then
       begin
-      increment_counter ictr;
+      increment_seqn (fun _ -> True) ictr;
       m_recall ctr;
       Some (Entry.p (Seq.index log j))
       end
